compiler/backend/gc/generational_gcScript.sml
@@ -39,6 +39,7 @@ val gc_move_def = Define `
 val gc_move_consts = prove(
   ``!x x' state state'.
     (gc_move conf state x = (x',state')) ==>
+    (state.old = state'.old) /\
     (state.h1 = state'.h1) /\
     (state.r3 = state'.r3) /\
     (state.r2 = state'.r2) /\
@@ -70,6 +71,7 @@ val gc_move_list_consts = prove(
   ``!xs xs' state state'.
     (gc_move_list conf state xs = (xs',state')) ==>
     (LENGTH xs = LENGTH xs') /\
+    (state.old = state'.old) /\
     (state.h1 = state'.h1) /\
     (state.r3 = state'.r3) /\
     (state.r2 = state'.r2) /\
@@ -104,6 +106,29 @@ val gc_move_data_def = tDefine "gc_move_data"  `
   \\ imp_res_tac (GSYM gc_move_list_consts)
   \\ fs []
   \\ decide_tac)
+
+val gc_move_data_consts = prove(
+  ``!state state'.
+    (gc_move_data conf state = state') ==>
+    (state.old = state'.old) /\
+    (state.r1 = state'.r1)
+  ``,
+  cheat);
+  (* rpt gen_tac *)
+  (* \\ Induct_on `state.h2` \\ fs [] *)
+  (* \\ once_rewrite_tac [gc_move_data_def] *)
+  (* \\ rpt strip_tac *)
+  (* \\ qpat_x_assum `_ = state.h2` (assume_tac o GSYM) *)
+  (* \\ fs [] *)
+  (* \\ Cases_on `conf.limit < heap_length (state.h1 ++ h::v)` \\ fs [] *)
+  (* >- fs [gc_state_component_equality] *)
+  (* \\ Cases_on `h` \\ fs [] *)
+  (* >- fs [gc_state_component_equality] *)
+  (* >- fs [gc_state_component_equality] *)
+  (* \\ pairarg_tac \\ fs [] *)
+  (* \\ drule gc_move_list_consts \\ strip_tac *)
+  (* \\ res_tac *)
+
 
 val gc_move_refs_def = tDefine "gc_move_refs" `
   (* maybe more refs (r4 could have more) *)
@@ -143,45 +168,45 @@ val partial_gc_def = Define `
       let n = heap_length current in
       let state = empty_state
           with <| heap := heap
+                ; old := old
                 ; r2 := refs
                 ; a := conf.gen_start; n := n |> in
         (* process roots: *)
       let (roots,state) = gc_move_list conf state roots in
-        (* process roots from references: *)
+        (* process references: *)
       let state = gc_move_refs conf state in
         (* process rest: *)
-      let state = gc_move_loop conf state conf.limit in
+      let state = gc_move_data conf state in
       (* let ok = ok0 /\ state.ok /\ *)
       (*          (state.a = conf.gen_start + heap_length state.h1) /\ *)
       (*          (state.r = heap_length state.r1) /\ *)
       (*          (heap_length state.heap = conf.limit) /\ *)
       (*          (state.a + state.n + state.r = conf.limit) /\ *)
       (*          state.a + state.r <= conf.limit in *)
-      let state = state with <|h1 := old ++ state.h1|> in
-      (roots,state)`; (* TODO: old? *)
+      (roots,state)`;
 
-val full_gc_def = Define `
-  full_gc conf (roots,heap) =
-    partial_gc
-      (conf with <| gen_start := 0; gen_end := conf.limit; refs_start := conf.limit |>)
-      (roots,heap)`;
+(* val full_gc_def = Define ` *)
+(*   full_gc conf (roots,heap) = *)
+(*     partial_gc *)
+(*       (conf with <| gen_start := 0; gen_end := conf.limit; refs_start := conf.limit |>) *)
+(*       (roots,state)`; *)
 
 (* Pointers between current and old generations are correct *)
 val heap_gen_ok_def = Define `
   heap_gen_ok heap conf =
     ?old current refs.
-      (SOME (old, current, refs) = heap_segment (conf.gen_start, conf.gen_end) heap) /\
+      (SOME (old, current, refs) = heap_segment (conf.gen_start, conf.refs_start) heap) /\
       (* old points only to itself and references *)
       (!ptr xs l d u. MEM (DataElement xs l d) old /\ MEM (Pointer ptr u) xs ==>
-        (ptr < conf.gen_start \/ conf.gen_end <= ptr)) /\
+        (ptr < conf.gen_start \/ conf.refs_start <= ptr)) /\
       (* old contains no references *)
       (!xs l d. MEM (DataElement xs l d) old ==> ~ (conf.isRef d)) /\
       (* refs only contains references *)
       (!xs l d. MEM (DataElement xs l d) refs ==> conf.isRef d)`;
 
 val _ = Datatype `
-  data_sort = Protected 'a      (* actually a pointer to an older generation *)
-            | Real 'b`;         (* a pointer to current generation/data *)
+  data_sort = Protected 'a      (* pointer to old generations *)
+            | Real 'b`;         (* data or pointer to current generation *)
 
 val to_basic_heap_address_def = Define `
   (to_basic_heap_address conf (Data a) = Data (Real a)) /\
@@ -193,14 +218,14 @@ val to_basic_heap_address_def = Define `
     else
       Pointer (ptr - conf.gen_start) (Real a))`;
 
-val to_gen_heap_address_def = Define `
-  (to_gen_heap_address gen_start (Data (Protected a)) = a) /\
-  (to_gen_heap_address gen_start (Data (Real b)) = Data b) /\
-  (to_gen_heap_address gen_start (Pointer ptr (Real a)) = Pointer (ptr + gen_start) a)`;
+(* val to_gen_heap_address_def = Define ` *)
+(*   (to_gen_heap_address gen_start (Data (Protected a)) = a) /\ *)
+(*   (to_gen_heap_address gen_start (Data (Real b)) = Data b) /\ *)
+(*   (to_gen_heap_address gen_start (Pointer ptr (Real a)) = Pointer (ptr + gen_start) a)`; *)
 
 val to_basic_conf_def = Define `
   to_basic_conf (conf:'a gen_gc_conf) =
-    <| limit := conf.limit
+    <| limit := conf.limit - conf.gen_start - (conf.limit - conf.refs_start)
      ; isRef := conf.isRef |>
      : 'a basic_gc_conf`;
 
@@ -211,12 +236,6 @@ val to_basic_heap_element_def = Define `
   (to_basic_heap_element conf (DataElement ptrs l d) =
     DataElement (MAP (to_basic_heap_address conf) ptrs) l d)`;
 
-val restrict_heap_def = Define `
-  restrict_heap start end (heap:('a,'b) heap_element list) =
-     case heap_segment (start,end) heap of
-     | NONE => ARB
-     | SOME (h1,h2,h3) => h2`;
-
 val to_basic_heap_list_def = Define `
   to_basic_heap_list conf heap =
     MAP (to_basic_heap_element conf) heap`;
@@ -224,17 +243,17 @@ val to_basic_heap_list_def = Define `
 val to_basic_heap_def = Define `
   to_basic_heap conf heap =
     to_basic_heap_list conf
-        (restrict_heap conf.gen_start conf.refs_start heap)`;
+        (heap_restrict conf.gen_start conf.refs_start heap)`;
 
 val to_basic_state_def = Define `
   to_basic_state conf state =
     empty_state with
     <| h1 := to_basic_heap_list conf state.h1
      ; h2 := to_basic_heap_list conf state.h2
-     ; r4 := to_basic_heap_list conf state.r4
-     ; r3 := to_basic_heap_list conf state.r3
-     ; r2 := to_basic_heap_list conf state.r2
-     ; r1 := to_basic_heap_list conf state.r1
+     ; r4 := []
+     ; r3 := []
+     ; r2 := []
+     ; r1 := []
      ; a := state.a - conf.gen_start
      ; n := state.n
      ; ok := state.ok
@@ -242,64 +261,19 @@ val to_basic_state_def = Define `
      ; heap0 := to_basic_heap conf state.heap0
      |>`;
 
-(* val roots_shift_def = Define ` *)
-(*   (roots_shift gen_start (Data a) = Data (Real a)) /\ *)
-(*   (roots_shift gen_start (Pointer ptr a) = *)
-(*     if ptr < gen_start then (Data (Protected (Pointer ptr a))) *)
-(*     else Pointer (ptr - gen_start) (Real a))`; *)
-
 val to_basic_roots_def = Define `
   to_basic_roots conf roots =
     MAP (to_basic_heap_address conf) roots`;
 
-val r2r_filter_def = Define `
-  (r2r_filter (Pointer _ _) = T) /\
-  (r2r_filter _ = F)`;
+(* val r2r_filter_def = Define ` *)
+(*   (r2r_filter (Pointer _ _) = T) /\ *)
+(*   (r2r_filter _ = F)`; *)
 
 val refs_to_roots_def = Define `
   (refs_to_roots conf [] = []) /\
   (refs_to_roots conf (DataElement ptrs _ _::refs) =
     MAP (to_basic_heap_address conf) ptrs ++ refs_to_roots conf refs) /\
   (refs_to_roots conf (_::refs) = refs_to_roots conf refs)`;
-
-(* val (RootsRefs_def,RootsRefs_ind,RootsRefs_cases) = Hol_reln ` *)
-(*   (RootsRefs [] []) /\ *)
-(*   (!ptrs m b refs roots ptr a ptr' a'. *)
-(*      RootsRefs (DataElement ptrs m b::refs) roots ==> *)
-(*      RootsRefs (DataElement (Pointer ptr a::ptrs) m b::refs) (Pointer ptr' a'::roots)) /\ *)
-(*   (!ptrs m b refs roots a. *)
-(*      RootsRefs (DataElement ptrs m b::refs) roots ==> *)
-(*      RootsRefs (DataElement (Data a::ptrs) m b::refs) roots) /\ *)
-(*   (!refs roots m b. *)
-(*      RootsRefs refs roots ==> *)
-(*      RootsRefs (DataElement [] m b::refs) roots) /\ *)
-(*   (!ptrs m b refs a. *)
-(*      RootsRefs (DataElement ptrs m b::refs) [] ==> *)
-(*      RootsRefs (DataElement (Data a::ptrs) m b::refs) []) /\ *)
-(*   (!refs roots n. *)
-(*      RootsRefs refs roots ==> *)
-(*      RootsRefs (Unused n::refs) roots) /\ *)
-(*   (!refs roots. *)
-(*      RootsRefs refs roots ==> *)
-(*      RootsRefs (ForwardPointer _ _ _::refs) roots)`; *)
-
-(* val RootsRefs_related = prove( *)
-(*   ``!refs. RootsRefs refs (refs_to_roots refs)``, *)
-(*   Induct *)
-(*   >- (simp [refs_to_roots_def] *)
-(*      \\ metis_tac [RootsRefs_cases]) *)
-(*   \\ Cases *)
-(*   \\ simp [refs_to_roots_def] *)
-(*   >- metis_tac [RootsRefs_cases] *)
-(*   >- metis_tac [RootsRefs_cases] *)
-(*   \\ Induct_on `l` *)
-(*   \\ simp [] *)
-(*   >- metis_tac [RootsRefs_cases] *)
-(*   \\ Cases *)
-(*   >- (simp [r2r_filter_def] *)
-(*      \\ metis_tac [RootsRefs_cases]) *)
-(*   \\ simp [r2r_filter_def] *)
-(*   \\ metis_tac [RootsRefs_cases]); *)
 
 (*
 
@@ -313,38 +287,21 @@ out    o ----> o
 last step: need a relation <---
  *)
 
+val heap_element_is_ref_def = Define `
+  (heap_element_is_ref conf (DataElement xs l d) = conf.isRef d) /\
+  (heap_element_is_ref conf _ = F)`;
+
 val gen_inv_def = Define `
   gen_inv (conf:'b gen_gc_conf) heap =
-    !h1 h2 h3 (* h10 h20 h30 *).
-    (heap_segment (conf.gen_start,conf.refs_start) heap = SOME (h1,h2,h3))(*  /\ *)
-    (* (heap_segment (conf.gen_start,conf.refs_start) state.heap0 = SOME (h10,h20,h30)) *)`;
+    conf.gen_start <= conf.refs_start /\
+    conf.refs_start <= conf.limit /\
+    ?heap_old heap_current heap_refs.
+    (heap_segment (conf.gen_start,conf.refs_start) heap = SOME (heap_old,heap_current,heap_refs)) /\
+    EVERY (λe. ¬heap_element_is_ref conf e) heap_old /\
+    EVERY (λe. ¬heap_element_is_ref conf e) heap_current`;
 
-(* val gc_forward_ptr_gen_inv = prove( *)
-(*   ``!state state' conf n ptr a ok. *)
-(*     gen_inv conf state /\ *)
-(*     (gc_forward_ptr n state.heap ptr a state.ok = (heap',ok')) ==> *)
-(*     gen_inv conf (state with <|heap:=heap';ok:=ok'|>)``, *)
-(*   cheat); *)
-(*   (* Induct_on `state.heap` *) *)
-(*   (* \\ rw [] *) *)
-(*   (* \\ qpat_x_assum `_ = state.heap` (assume_tac o GSYM) \\ fs [] *) *)
-(*   (* \\ fs [gc_forward_ptr_def,gen_inv_def] *) *)
-(*   (* \\ qpat_x_assum `_ = (heap',ok')` mp_tac *) *)
-(*   (* \\ IF_CASES_TAC \\ fs [] *) *)
-(*   (* >- (strip_tac *) *)
-(*   (*    \\ qpat_x_assum `_ = heap'` (assume_tac o GSYM) \\ fs [] *) *)
-(*   (*    \\ rpt strip_tac *) *)
-(*   (*    \\ fs [heap_segment_def,heap_split_def,el_length_def] *) *)
-(*   (*    \\ fs []) *) *)
-(*   (* cheat); *) *)
-
-(* val gc_move_heap_lookup_lemma = prove( *)
-(*   ``!heap n conf. *)
-(*     ¬(n < conf.gen_start) /\ *)
-(*     ¬(conf.refs_start ≤ n) /\ *)
-(*     (heap_lookup (n − conf.gen_start) (to_basic_state conf state).heap *)
-(*      = OPTION_MAP ()) ==> *)
-(*     (heap_lookup n state.heap = NONE) *)
+(* always rewrite with gen_inv_def *)
+val _ = augment_srw_ss [rewrites [gen_inv_def]];
 
 val gc_move_simulation = prove(
   ``!ptr ptr' state state'.
@@ -357,27 +314,28 @@ val gc_move_simulation = prove(
          (to_basic_heap_address conf ptr)
        = (to_basic_heap_address conf ptr', to_basic_state conf state'))``,
   reverse Cases
-  \\ ntac 4 strip_tac
+  \\ fs []
+  \\ rpt gen_tac
+  \\ strip_tac
   \\ fs [to_basic_heap_address_def]
   >- (fs [gc_move_def,basic_gcTheory.gc_move_def]
-     \\ qpat_x_assum `Data a = _` (assume_tac o GSYM)
+     \\ rveq
+     \\ fs [to_basic_heap_address_def])
+  \\ fs []
+  \\ IF_CASES_TAC
+  >- (fs [gc_move_def,basic_gcTheory.gc_move_def]
+     \\ rveq
      \\ fs [to_basic_heap_address_def])
   \\ IF_CASES_TAC
-  >- (fs [gc_move_def,basic_gcTheory.gc_move_def,gen_inv_def]
-     \\ qpat_x_assum `_ = ptr'` (assume_tac o GSYM) \\ fs []
+  >- (fs [gc_move_def,basic_gcTheory.gc_move_def]
+     \\ rveq
      \\ fs [to_basic_heap_address_def])
-  \\ IF_CASES_TAC
-  >- (fs [gc_move_def,basic_gcTheory.gc_move_def,gen_inv_def]
-     \\ qpat_x_assum `_ = ptr'` (assume_tac o GSYM) \\ fs []
-     \\ fs [to_basic_heap_address_def])
-  \\ fs [gen_inv_def]
-  \\ qpat_x_assum `!h1. _` (assume_tac o SPEC_ALL)
   \\ fs [gc_move_def,basic_gcTheory.gc_move_def]
   \\ strip_tac >- cheat
   \\ BasicProvers.TOP_CASE_TAC \\ fs []
   >- (`heap_lookup n state.heap = NONE` by all_tac
      >- (pop_assum mp_tac
-        \\ fs [to_basic_state_def,to_basic_heap_def,restrict_heap_def]
+        \\ fs [to_basic_state_def,to_basic_heap_def,heap_restrict_def]
         \\ fs [heap_lookup_def]
         \\ cheat
      )
@@ -394,54 +352,53 @@ val gc_move_list_simulation = prove(
     = (MAP (to_basic_heap_address conf) xs', to_basic_state conf state'))``,
   cheat);
 
-(* val fmap_fun_def = Define ` *)
-(*   fmap_fun (f:num |-> num) gen_start heap = *)
-(*     FUN_FMAP (\n. if n < gen_start then n else $FAPPLY f (n - gen_start) + gen_start) *)
-(*              ({n | n < gen_start /\ n IN heap_addresses 0 heap} *)
-(*               UNION IMAGE (\n. n + gen_start) (FDOM f))`; *)
+val gc_move_list_simulation = prove(
+  ``!state0 roots0 roots1 state1.
+    (gc_move_list conf state0 roots0 = (roots1,state1))
+    ==>
+    (gc_move_list (to_basic_conf conf)
+      (to_basic_state conf state0) (to_basic_roots conf roots0) =
+        (to_basic_roots conf roots1,to_basic_state conf state1))``,
+  cheat);
 
-(* val fmap_fun_finite = store_thm("fmap_fun_finite[simp]", *)
-(*   ``FINITE ({n | n < gen_start ∧ n ∈ heap_addresses 0 heap} ∪ *)
-(*            IMAGE (λn'. gen_start + n') (FDOM f))``, *)
-(*   rewrite_tac [FINITE_UNION] *)
-(*   \\ fs [] *)
-(*   \\ Induct_on `gen_start` *)
-(*   \\ fs [] *)
-(*   \\ `{n | n < SUC gen_start ∧ n ∈ heap_addresses 0 heap} = *)
-(*       if gen_start IN heap_addresses 0 heap *)
-(*       then gen_start INSERT {n | n < gen_start ∧ n ∈ heap_addresses 0 heap} *)
-(*       else {n | n < gen_start ∧ n ∈ heap_addresses 0 heap}` by all_tac *)
-(*   >- (cheat)(* EXTENSION *) *)
-(*   \\ fs [] *)
-(*   \\ rw []); *)
+val gc_move_list_APPEND = prove(
+  ``!conf state0 xs ys roots' state'.
+  (basic_gc$gc_move_list conf state0 (xs ++ ys) = (roots',state')) ==>
+  ?roots1 roots2 state1.
+  (basic_gc$gc_move_list conf state0 xs = (roots1,state1)) /\
+  (basic_gc$gc_move_list conf state1 ys = (roots2,state')) /\
+  (roots' = roots1 ++ roots2)``,
+  cheat);
 
-(* val addr_map_take = prove( *)
-(*   ``!n f xs. TAKE n (ADDR_MAP f xs) = ADDR_MAP f (TAKE n xs)``, *)
-(*   Induct *)
-(*   >- fs [TAKE_def,ADDR_MAP_def] *)
-(*   \\ Cases_on `xs` *)
-(*   \\ fs [TAKE_def,ADDR_MAP_def] *)
-(*   \\ Cases_on `h` *)
-(*   \\ fs [TAKE_def,ADDR_MAP_def]); *)
+val heap_restrict_NIL = store_thm("heap_restrict_NIL[simp]",
+  ``heap_restrict gen_start refs_start [] = []``,
+  cheat);
 
-val roots_ok_TL = prove(
-    ``roots_ok (h::roots) heap ==> roots_ok roots heap``, cheat);
+val to_basic_heap_NIL = store_thm("to_basic_heap_NIL[simp]",
+  ``to_basic_heap conf [] = []``,
+  cheat);
 
-val fmap_fun_LESS_gen_start = prove(
-  ``n IN heap_addresses 0 heap /\ n < gen_start ==>
-    (fmap_fun f gen_start heap ' n = n)``,
-  fs [fmap_fun_def,FUN_FMAP_DEF]);
+val to_basic_heap_list_NIL = store_thm("to_basic_heap_list_NIL[simp]",
+  ``to_basic_heap_list conf [] = []``,
+  cheat);
 
-val heap_element_is_ref_def = Define `
-  (heap_element_is_ref conf (DataElement xs l d) = conf.isRef d) /\
-  (heap_element_is_ref conf _ = F)`;
+val gc_move_list_refs_lemma = prove(
+  ``!state state1.
+    (gc_move_refs conf state = state1) ==>
+    (gc_move_list (to_basic_conf conf) (to_basic_state conf state)
+        (refs_to_roots conf state.r2) =
+     (refs_to_roots conf state1.r1,to_basic_state conf state1))
+  ``,
+  cheat) |> SIMP_RULE std_ss [];
 
 val partial_gc_simulation = prove(
   ``!roots heap0 roots1 state1 heap0_old heap0_current heap0_refs.
     (partial_gc conf (roots,heap0) = (roots1,state1)) /\
     heap_gen_ok heap0 conf /\
-    (SOME (heap0_old,heap0_current,heap0_refs) = heap_segment (conf.gen_start,conf.refs_start) heap0) /\
-    EVERY (\e. ~(heap_element_is_ref conf e)) (heap0_old ++ heap0_start) /\
+    conf.gen_start ≤ conf.refs_start ∧ conf.refs_start ≤ conf.limit /\
+    (SOME (heap0_old,heap0_current,heap0_refs) =
+      heap_segment (conf.gen_start,conf.refs_start) heap0) /\
+    EVERY (\e. ~(heap_element_is_ref conf e)) (heap0_old ++ heap0_current) /\
     roots_ok roots heap0 /\
     heap_ok heap0 conf.limit ==>
     ?refs refs1.
